Repair env-based thunkLang

compiler/backend/thunkLangScript.sml
@@ -18,15 +18,13 @@ val _ = new_theory "thunkLang";
 
 val _ = numLib.prefer_num();
 
-Type vname = “:string”;
-Type op = “:pure_exp$op”;
-
 Datatype:
   exp = Var vname                                (* variable                *)
       | Prim op (exp list)                       (* primitive operations    *)
       | App exp exp                              (* function application    *)
       | Lam vname exp                            (* lambda                  *)
-      | Letrec ((vname # vname # exp) list) exp  (* mutually recursive exps *)
+      | Letrec ((vname #  exp) list) exp         (* mutually recursive exps *)
+      | Let vname exp exp                        (* non-recursive let       *)
       | If exp exp exp                           (* if-then-else            *)
       | Delay exp                                (* suspend in a Thunk      *)
       | Box exp                                  (* wrap result in a Thunk  *)
@@ -36,34 +34,22 @@ End
 Datatype:
   v = Constructor string (v list)
     | Closure vname ((vname # v) list) exp
-    | Recclosure ((vname # vname # exp) list) ((vname # v) list) vname
+    | Recclosure ((vname # exp) list) ((vname # v) list) vname
     | Thunk (v + (vname # v) list # exp)
     | Atom lit
 End
 
-Definition bind_funs_def:
+Definition bind_funs_def[simp]:
   bind_funs funs env =
     MAP (λ(fn, _). (fn, Recclosure funs env fn)) funs ++ env
 End
 
-Definition dest_Closure_def:
+Definition dest_Closure_def[simp]:
   dest_Closure (Closure s env x) = return (s, env, x) ∧
   dest_Closure _ = fail Type_error
 End
 
-Definition dest_Thunk_def:
-  dest_Thunk (Thunk x) = return x ∧
-  dest_Thunk _ = fail Type_error
-End
-
-Definition lookup_var_def:
-  lookup_var env x =
-    case ALOOKUP env x of
-      NONE => fail Type_error
-    | SOME v => return v
-End
-
-Definition dest_Recclosure_def:
+Definition dest_Recclosure_def[simp]:
   dest_Recclosure (Recclosure funs env fn) = return (funs, env, fn) ∧
   dest_Recclosure _ = fail Type_error
 End
@@ -72,13 +58,34 @@ Definition dest_anyClosure_def:
   dest_anyClosure v =
     dest_Closure v ++
     do
-      (funs, env, fn) <- dest_Recclosure v;
-      (var, bod) <- lookup_var funs fn ;
-      return (var, bind_funs funs env, bod)
+      (f, env, n) <- dest_Recclosure v;
+      case ALOOKUP (REVERSE f) n of
+        SOME (Lam s x) => return (s, bind_funs f env, x)
+      | _ => fail Type_error
     od
 End
 
-Definition dest_Constructor_def:
+Definition dest_Thunk_def[simp]:
+  dest_Thunk (Thunk x) = return x ∧
+  dest_Thunk _ = fail Type_error
+End
+
+Definition dest_anyThunk_def:
+  dest_anyThunk v =
+    do
+      w <- dest_Thunk v;
+      return (w, [])
+    od ++
+    do
+      (f, env, n) <- dest_Recclosure v;
+      case ALOOKUP (REVERSE f) n of
+        SOME (Delay x) => return (INR (env, x), f)
+      | SOME (Box x) => return (INR (env, x), f)
+      | _ => fail Type_error
+    od
+End
+
+Definition dest_Constructor_def[simp]:
   dest_Constructor (Constructor s vs) = return (s, vs) ∧
   dest_Constructor _ = fail Type_error
 End
@@ -88,7 +95,10 @@ Definition unit_def:
 End
 
 Definition eval_to_def:
-  eval_to k env (Var n) = lookup_var env n ∧
+  eval_to k env (Var n) =
+    (case ALOOKUP env n of
+       SOME v => return v
+     | NONE => fail Type_error) ∧
   eval_to k env (App f x) =
     (do
        fv <- eval_to k env f;
@@ -97,6 +107,12 @@ Definition eval_to_def:
        if k = 0 then fail Diverge else eval_to (k - 1) ((s, xv)::env) body
      od) ∧
   eval_to k env (Lam s x) = return (Closure s env x) ∧
+  eval_to k env (Let n x y) =
+    (if k = 0 then fail Diverge else
+       do
+         v <- eval_to (k - 1) env x;
+         eval_to (k - 1) ((n, v)::env) y
+       od) ∧
   eval_to k env (If x y z) =
     (if k = 0 then fail Diverge else
        do
@@ -126,11 +142,10 @@ Definition eval_to_def:
        | INR (env, y) => if k = 0 then fail Diverge else eval_to (k - 1) env y
      od) ∧
   eval_to k env (Prim op xs) =
-    (if k = 0 then fail Diverge else
-       case op of
-         Cons s =>
+    (case op of
+       Cons s =>
            do
-             vs <- map (eval_to (k - 1) env) xs;
+             vs <- map (λx. eval_to k env x) xs;
              return (Constructor s vs)
            od
        | If => fail Type_error
@@ -138,7 +153,7 @@ Definition eval_to_def:
        | Proj s i =>
            do
              assert (LENGTH xs = 1);
-             v <- eval_to (k - 1) env (HD xs);
+             v <- if k = 0 then fail Diverge else eval_to (k - 1) env (HD xs);
              (t, ys) <- dest_Constructor v;
              assert (t = s ∧ i < LENGTH ys);
              return (EL i ys)
@@ -146,17 +161,18 @@ Definition eval_to_def:
        | IsEq s i =>
            do
              assert (LENGTH xs = 1);
-             v <- eval_to (k - 1) env (HD xs);
+             v <- if k = 0 then fail Diverge else eval_to (k - 1) env (HD xs);
              (t, ys) <- dest_Constructor v;
              assert (t = s ⇒ i = LENGTH ys);
              return (Constructor (if t ≠ s then "False" else "True") [])
            od
        | AtomOp aop =>
            do
-             ys <- map (λx. case eval_to (k - 1) env x of
-                              INR (Atom l) => return l
-                            | INL e => fail e
-                            | _ => fail Type_error) xs;
+             ys <- map (λx. if k = 0 then fail Diverge else
+                              case eval_to (k - 1) env x of
+                                INR (Atom l) => return l
+                              | INL err => fail err
+                              | _ => fail Type_error) xs;
              case eval_op aop ys of
                SOME (INL v) => return (Atom v)
              | SOME (INR b) =>
@@ -164,7 +180,8 @@ Definition eval_to_def:
              | NONE => fail Type_error
            od)
 Termination
-  WF_REL_TAC ‘inv_image ($< LEX $<) (λ(k, c, x). (k, exp_size x))’
+  WF_REL_TAC ‘inv_image ($< LEX $<) (λ(k, c, x). (k, exp_size x))’ \\ rw []
+  \\ Induct_on ‘xs’ \\ rw [] \\ fs [fetch "-" "exp_size_def"]
 End
 
 Definition eval_def:
@@ -180,15 +197,18 @@ Definition freevars_def:
   freevars (If x y z)  = freevars x ∪ freevars y ∪ freevars z ∧
   freevars (App x y) = freevars x ∪ freevars y ∧
   freevars (Lam s b) = freevars b DIFF {s} ∧
-  freevars (Letrec f x) = ∅ (* TODO *) ∧
+  freevars (Let s x y) = freevars x ∪ (freevars y DIFF {s}) ∧
+  freevars (Letrec f x) =
+    ((freevars x ∪ BIGUNION (set (MAP (λ(n, x). freevars x) f))) DIFF
+     set (MAP FST f)) ∧
   freevars (Delay x) = freevars x ∧
   freevars (Box x) = freevars x ∧
   freevars (Force x) = freevars x
 Termination
   WF_REL_TAC ‘measure exp_size’
-  \\ fs [] \\ gen_tac
-  \\ Induct \\ rw []
-  \\ res_tac
+  \\ rw []
+  \\ rename1 ‘MEM _ xs’
+  \\ Induct_on ‘xs’ \\ rw []
   \\ fs [fetch "-" "exp_size_def"]
 End
 
@@ -218,6 +238,10 @@ Proof
     \\ IF_CASES_TAC \\ fs [])
   >- ((* Lam *)
     simp [eval_to_def])
+  >- ((* Let *)
+    rw [eval_to_def]
+    \\ Cases_on ‘eval_to (k - 1) env x’ \\ fs []
+    \\ IF_CASES_TAC \\ fs [])
   >- ((* If *)
     rename1 ‘If x y z’
     \\ rw [eval_to_def]
@@ -242,25 +266,26 @@ Proof
     dsimp []
     \\ strip_tac
     \\ strip_tac
+    \\ fs [MEM_EL, PULL_EXISTS]
     \\ Cases_on ‘op’ \\ rw [eval_to_def] \\ gs []
     >- ((* Cons *)
-      Cases_on ‘map (λx. eval_to (j - 1) env x) xs’ \\ fs []
+      Cases_on ‘map (λx. eval_to j env x) xs’ \\ fs []
       >- (
-        reverse (Cases_on ‘map (λx. eval_to (k - 1) env x) xs’) \\ fs []
+        reverse (Cases_on ‘map (λx. eval_to k env x) xs’) \\ fs []
         >- (
           fs [map_INL]
           \\ drule_then assume_tac map_INR
           \\ first_x_assum (drule_then assume_tac) \\ gs [])
         \\ gvs [map_INL]
-        \\ rename1 ‘eval_to (j - 1) env (EL m xs) = INL d’
-        \\ rename1 ‘eval_to (k - 1) env (EL n xs) = INL e’
+        \\ rename1 ‘eval_to j env (EL m xs)’
+        \\ rename1 ‘eval_to k env (EL n xs)’
         \\ Cases_on ‘m < n’ \\ gs []
         \\ Cases_on ‘m = n’ \\ gs []
         \\ ‘n < m’ by gs []
         \\ first_assum (drule_then assume_tac)
-        \\ ‘eval_to (k - 1) env (EL n xs) ≠ INL Diverge’ by fs []
-        \\ first_x_assum (drule_then (qspec_then ‘j - 1’ assume_tac)) \\ gs [])
-      \\ Cases_on ‘map (λx. eval_to (k - 1) env x) xs’ \\ fs []
+        \\ ‘eval_to k env (EL n xs) ≠ INL Diverge’ by fs []
+        \\ first_x_assum (drule_then assume_tac) \\ gs [])
+      \\ Cases_on ‘map (λx. eval_to k env x) xs’ \\ fs []
       >- (
         fs [map_INL]
         \\ drule_then assume_tac map_INR
@@ -288,18 +313,20 @@ Proof
         >- (
           fs [map_INL, Abbr ‘f’, Abbr ‘g’]
           \\ drule_all_then assume_tac map_INR
-          \\ gs [CaseEqs ["sum", "v"]])
+          \\ gs [CaseEqs ["sum", "v", "bool"]])
         \\ fs [map_INL, Abbr ‘f’, Abbr ‘g’]
-        \\ rename1 ‘sum_CASE (eval_to (j - 1) env (EL m xs)) _ _ = INL d’
-        \\ rename1 ‘sum_CASE (eval_to (k - 1) env (EL n xs)) _ _ = INL e’
+        \\ rename1 ‘eval_to (j - 1) env (EL m xs)’
+        \\ rename1 ‘eval_to (k - 1) env (EL n xs)’
         \\ Cases_on ‘m < n’ \\ gs []
         >- (
           first_x_assum (drule_then assume_tac)
-          \\ gs [CaseEq "sum"])
+          \\ gs [CaseEqs ["sum", "bool"]])
         \\ Cases_on ‘m = n’ \\ gs []
         >- (
-          gvs [CaseEq "sum"])
+          gvs [CaseEqs ["sum", "bool"]])
+        \\ gvs [CaseEq "bool"]
         \\ ‘n < m’ by gs []
+        \\ ‘n < LENGTH xs’ by gs []
         \\ first_assum (drule_then assume_tac)
         \\ ‘eval_to (k - 1) env (EL n xs) ≠ INL Diverge’ by (strip_tac \\ fs [])
         \\ first_x_assum (drule_then (qspec_then ‘j - 1’ mp_tac))
@@ -309,7 +336,7 @@ Proof
       >- (
         fs [map_INL, Abbr ‘f’, Abbr ‘g’]
         \\ drule_all_then assume_tac map_INR
-        \\ gs [CaseEq "sum"])
+        \\ gs [CaseEqs ["sum", "bool"]])
       \\ rename1 ‘map f _ = INR v’
       \\ rename1 ‘map g _ = INR w’
       \\ ‘v = w’ suffices_by rw []
@@ -317,6 +344,7 @@ Proof
       \\ first_assum (mp_then Any assume_tac map_INR)
       \\ last_assum (mp_then Any assume_tac map_INR)
       \\ unabbrev_all_tac
+      \\ Cases_on ‘k = 0’ \\ fs []
       \\ irule LIST_EQ \\ rw [] \\ gs [CaseEqs ["sum", "v"]]))
 QED
 
